(WIP) Typed expression evaluator for Verilog

vvequiv/Verilog.v
@@ -5,52 +5,114 @@ Import Bitvector (bv, mkBV).
 Require Import String.
 Require Import ZArith.
 Require Import BinNums.
+Require Import Psatz.
 
 Require Import List.
 Import ListNotations.
 From Coq Require Arith Lia Program.
+From Coq Require Import Setoid.
 From Equations Require Import Equations.
 
 (* This module will be Verilog.Verilog. Redundant, but it is needed for extraction. See Extraction.v *)
 Module Verilog.
-  Set Implicit Arguments.
-  Set Strict Implicit.
+  Inductive VType :=
+    | Logic (hi lo : N).
 
-  Inductive VType := Logic : N -> N -> VType.
+  (* Equations Derive NoConfusionHom EqDec for VType. *)
+  (* Next Obligation. *)
+  (*   destruct x as [hi1 lo1]. *)
+  (*   destruct y as [hi2 lo2]. *)
+  (*   destruct (N.eq_dec hi1 hi2); destruct (N.eq_dec lo1 lo2); subst. *)
+  (*   - left. reflexivity. *)
+  (*   - right. intros contra. inversion contra. *)
+  (*     auto. *)
+  (*   - right. intros contra. inversion contra. *)
+  (*     auto. *)
+  (*   - right. intros contra. inversion contra. *)
+  (*     auto. *)
+  (* Defined. *)
 
-  Equations Derive NoConfusionHom EqDec for VType.
-  Next Obligation.
-    destruct x as [hi1 lo1].
-    destruct y as [hi2 lo2].
-    destruct (N.eq_dec hi1 hi2); destruct (N.eq_dec lo1 lo2); subst.
-    - left. reflexivity.
-    - right. intros contra. inversion contra.
-      auto.
-    - right. intros contra. inversion contra.
-      auto.
-    - right. intros contra. inversion contra.
-      auto.
-  Defined.
+  Definition vt_width (t : VType) : positive :=
+    let (hi, lo) := t in
+    let hi' := N.max hi lo in
+    let lo' := N.min hi lo in
+    Pos.of_succ_nat (N.to_nat (hi' - lo')).
+
+  Definition vt_compatible (t1 t2 : VType) : Prop :=
+    vt_width t1 = vt_width t2.
+
+  Declare Scope vtype.
+  Delimit Scope vtype with vtype.
+
+  Notation "a ≈ b" := (vt_compatible a b) (at level 100) : vtype.
+
+  Theorem vt_compatible_refl : forall t, (t ≈ t)%vtype.
+  Proof. reflexivity. Qed.
+
+  Theorem vt_compatible_symmetry : forall t1 t2,
+      (t1 ≈ t2)%vtype ->
+      (t2 ≈ t1)%vtype.
+  Proof. intros. symmetry. assumption. Qed.
+
+  Theorem vt_compatible_trans : forall t1 t2 t3,
+      (t1 ≈ t2)%vtype ->
+      (t2 ≈ t3)%vtype ->
+      (t1 ≈ t3)%vtype.
+  Proof. intros. transitivity (vt_width t2); assumption. Qed.
+
+  Add Parametric Relation : VType vt_compatible
+          reflexivity proved by vt_compatible_refl
+          symmetry proved by vt_compatible_symmetry
+          transitivity proved by vt_compatible_trans
+      as vt_compatible_rel
+  .
+
+  Ltac crush_vtype :=
+    repeat match goal with
+      | t : VType |- _ => destruct t
+      end;
+    repeat match goal with
+      | e : (_ ≈ _)%vtype |- _ => unfold "≈"%vtype in e; simpl in e
+      end;
+    match goal with
+    | |- (_ ≈ _)%vtype => unfold "≈"%vtype; simpl
+    end; try lia.
 
   Inductive BinaryOperator := Plus | Minus.
 
-  (* Equations bv_type (idx : Type) (bv : ) *)
+  Set Implicit Arguments.
+
   Structure VerilogKind :=
     { t :> Type
-    ; bv_type : Bitvector.bv -> t
+    ; bv_type : bv -> t
+    ; types_compatible : t -> t -> Prop
+    ; convert_bv : t -> bv -> bv
+    ; convert_bv_correct : forall (ty : t) (v : bv),
+        types_compatible (bv_type (convert_bv ty v)) ty
     }.
 
-  Definition Typed : VerilogKind :=
-    {| t := VType
-    ; bv_type v := Verilog.Logic (N.pred (N.pos (Bitvector.width v))) 0
-    |}.
-
-  Definition Untyped : VerilogKind :=
-    {| t := unit
-    ; bv_type _ := tt
-    |}.
-
   Arguments bv_type {_} & _.
+  Arguments convert_bv {_} & _.
+
+  Program Definition Untyped : VerilogKind :=
+    {| t := unit
+    ; types_compatible _ _ := True
+    ; bv_type _ := tt
+    ; convert_bv _ v := v
+    |}.
+
+  Program Definition Typed : VerilogKind :=
+    {| t := VType
+    ; types_compatible t1 t2 := vt_width t1 = vt_width t2
+    ; bv_type v :=
+        Verilog.Logic (N.pred (N.pos (Bitvector.width v))) 0
+    ; convert_bv ty v :=
+        let width__ty := vt_width ty in
+        Bitvector.convert width__ty v
+    |}.
+  Next Obligation. lia. Qed.
+
+  Notation "a ∈ b" := (vt_compatible (@bv_type Typed a) b) (at level 100) : vtype.
 
   Inductive Expression (k : VerilogKind) : k -> Type :=
   | BinaryOp :
@@ -80,6 +142,8 @@ Module Verilog.
   Notation TypedIntegerLiteral t v := (IntegerLiteral Typed t v).
   Notation UntypedIntegerLiteral v := (IntegerLiteral Untyped tt v).
 
+  Set Strict Implicit.
+
   Inductive Statement (k : VerilogKind) :=
   | Block (body : list (Statement k))
   | BlockingAssign {t : k} (lhs rhs : Expression k t)
@@ -98,20 +162,101 @@ Module Verilog.
       ; portName : string
       }.
 
-  Record Var :=
-    MkVar
-      { varType : VType
-      ; varName : string
-      }.
-
   (** Verilog modules *)
   Record VerilogModule (k: VerilogKind) :=
     MkVerilogModule
       { modName : string
       ; modPorts : list Port
-      ; modVariables : list Var
+      ; modVariables : StrMap.t VType
       ; modBody : list (ModuleItem k)
       }.
+
+  Record VerilogState k (m : VerilogModule k) :=
+    MkVerilogState
+      { blockingState : StrMap.t bv
+      (* ; nonblockingState : StrMap.t bv *)
+      ; blockingState_wf : forall n t (v : bv),
+          StrMap.MapsTo n t (modVariables m) ->
+          exists v, StrMap.MapsTo n v blockingState /\ (v ∈ t)%vtype
+      }
+  .
+
+  Unset Implicit Arguments.
+  Unset Strict Implicit.
+
+  Module TypedSemantics.
+    Equations compute_bin_op {t} :
+      BinaryOperator ->
+      {v : bv | (v ∈ t)%vtype} ->
+      {v : bv | (v ∈ t)%vtype} ->
+      {v : bv | (v ∈ t)%vtype} :=
+      (* TODO:
+    Can/should we unify the behaviour of typed and untyped verilog here?
+    - In typed verilog, we should have a proof that the operands are of the same width.
+    - In untyped verilog, we need context sensitivity, adding conversions if needed
+    - Perhaps we just need to split typed/untyped expression evaluation.
+      The rest of the interpreter can be shared
+       *)
+      compute_bin_op Plus (exist _ v1 prf1) (exist _ v2 prf2) :=
+        exist _ (Bitvector.bv_add_truncate v1 v2 _) _;
+      (* TODO: Operations other than add *)
+      compute_bin_op _ (exist _ v1 _) _ := exist _ v1 _
+    .
+    Next Obligation.
+      unfold vt_compatible in *.
+      simpl in *.
+      rewrite <- prf1 in *; clear prf1.
+      lia.
+    Qed.
+    Next Obligation.
+      rewrite (Bitvector.bv_add_truncate_width v1 v2).
+      trivial.
+    Qed.
+
+    Program Definition get_var {k} {m : VerilogModule k}
+      (st : VerilogState m)
+      (n : string)
+      (name_present : StrMap.In n (blockingState st)) :
+      { v : bv | StrMap.MapsTo n v (blockingState st) } :=
+      (match StrMap.find n (blockingState st) as r return (StrMap.find n (blockingState st) = r -> { v : bv | StrMap.MapsTo n v (blockingState st) }) with
+       | Some x => fun _ => (@exist _ _ x _)
+       | None => fun eq => _
+       end) eq_refl
+    .
+    Next Obligation.
+      rewrite StrMapFacts.find_mapsto_iff.
+      assumption.
+    Qed.
+    Next Obligation.
+      rewrite <- StrMapFacts.not_find_in_iff in *.
+      contradiction.
+    Qed.
+
+    Program Fixpoint eval_expression_typed {t : Typed} {m : VerilogModule Typed}
+      (st : VerilogState m)
+      (expr : Expression Typed t) :
+      {v : bv | (@bv_type Typed v ≈ t)%vtype} :=
+      match expr with
+      | BinaryOp op lhs rhs =>
+          compute_bin_op op
+            (eval_expression_typed st lhs)
+            (eval_expression_typed st rhs)
+      | Conversion to_type operand =>
+          let (val, prf) := (eval_expression_typed st operand) in
+          exist _ (convert_bv to_type val) _
+      | IntegerLiteral _ value =>
+          exist _ value _
+      | VarRef _ t n =>
+          let (v, prf) := get_var st n _ in
+          exist _ v _
+      end
+    .
+    Next Obligation. crush_vtype. Qed.
+    Next Obligation. reflexivity. Qed.
+    Next Obligation. (* n is present *) Admitted.
+    Next Obligation. (* VarRefs types match declaration, declarations match state *) Admitted.
+
+  End TypedSemantics.
 
   Example examples : list (VerilogModule Untyped * VerilogModule Untyped) :=
     let l32 := Logic 31 0 in
@@ -123,10 +268,10 @@ Module Verilog.
             MkPort PortIn "in" ;
             MkPort PortOut "out"
           ];
-          modVariables := [
-            MkVar l32 "in" ;
-            MkVar l32 "out"
-          ];
+          modVariables := StrMap.from_list [
+                              ("in"%string, l32);
+                              ("out"%string, l32)
+                            ];
           modBody := [
             ContinuousAssign
               (UntypedVarRef "out")
@@ -139,10 +284,10 @@ Module Verilog.
             MkPort PortIn "in" ;
             MkPort PortOut "out"
           ];
-          modVariables := [
-            MkVar l32 "in" ;
-            MkVar l32 "out"
-          ];
+          modVariables := StrMap.from_list [
+                              ("in"%string, l32) ;
+                              ("out"%string, l32)
+                            ];
           modBody := [
             ContinuousAssign
               (UntypedVarRef "out")
@@ -157,10 +302,10 @@ Module Verilog.
             MkPort PortIn "in" ;
             MkPort PortOut "out"
           ];
-          modVariables := [
-            MkVar l32 "in" ;
-            MkVar l32 "out"
-          ];
+          modVariables := StrMap.from_list [
+                              ("in"%string, l32) ;
+                              ("out"%string, l32)
+                            ];
           modBody := [
             ContinuousAssign
               (UntypedVarRef "out")
@@ -175,10 +320,10 @@ Module Verilog.
             MkPort PortIn "in" ;
             MkPort PortOut "out"
           ];
-          modVariables := [
-            MkVar l32 "in" ;
-            MkVar l32 "out"
-          ];
+          modVariables := StrMap.from_list [
+                              ("in"%string, l32) ;
+                              ("out"%string, l32)
+                            ];
           modBody := [
             ContinuousAssign
               (UntypedVarRef "out")
@@ -196,12 +341,12 @@ Module Verilog.
             MkPort PortIn "in2" ;
             MkPort PortOut "out"
           ];
-          modVariables := [
-            MkVar l32 "in1" ;
-            MkVar l32 "in2" ;
-            MkVar l16 "v" ;
-            MkVar l32 "out"
-          ];
+          modVariables := StrMap.from_list [
+                              ("in1"%string, l32) ;
+                              ("in2"%string, l32) ;
+                              ("v"%string, l16) ;
+                              ("out"%string, l32)
+                            ];
           modBody := [
             ContinuousAssign
               (UntypedVarRef "v")
@@ -222,11 +367,11 @@ Module Verilog.
             MkPort PortIn "in2" ;
             MkPort PortOut "out"
           ];
-          modVariables := [
-            MkVar l32 "in1" ;
-            MkVar l32 "in2" ;
-            MkVar l32 "out"
-          ];
+          modVariables := StrMap.from_list [
+                              ("in1"%string, l32) ;
+                              ("in2"%string, l32) ;
+                              ("out"%string, l32)
+                            ];
           modBody := [
             ContinuousAssign
               (UntypedVarRef "out")
